splitting aeh into fsti and fst

steel/Zeta.Steel.AggregateEpochHashes.fsti
@@ -20,10 +20,12 @@ open Zeta.Steel.Util
 module MR = Steel.ST.MonotonicReference
 module TLM = Zeta.Steel.ThreadLogMap
 open Zeta.Steel.EpochHashes
+
 #push-options "--ide_id_info_off"
 
-/// Initializer for an IArray
-val epoch_hash_size : U32.t
+
+//AR: TODO: This val is not used anywhere?
+//val epoch_hash_size : U32.t
 
 let tid_bitmap = Seq.lseq bool (U32.v n_threads)
 let epoch_hashes_repr = EpochMap.repr M.epoch_hash
@@ -164,96 +166,6 @@ type aggregate_epoch_hashes = {
      mlogs: TLM.t;
      lock: cancellable_lock (lock_inv hashes tid_bitmaps max_certified_epoch mlogs)
 }
-#push-options "--print_effect_args"
-
-let check_all_ones (#e:Ghost.erased _)
-                   (a:larray bool n_threads)
-  : ST bool
-    (array_pts_to a e)
-    (fun _ -> array_pts_to a e)
-    (requires True)
-    (ensures fun b -> b <==> (reveal e == all_ones))
-  = admit__()
-
-let return_borrows (#v:Type0) (b:EpochMap.borrows v) (i:M.epoch_id) (x:v)
-  : Lemma (requires ~(PartialMap.contains b i))
-          (ensures (PartialMap.remove (PartialMap.upd b i x) i `PartialMap.equal` b))
-          [SMTPat (PartialMap.remove (PartialMap.upd b i x) i)]
-  = ()
-
-let return_map (#v:Type0) (m:EpochMap.repr v) (i:M.epoch_id)
-  : Lemma (ensures (Map.upd m i (Map.sel m i) `Map.equal` m))
-          [SMTPat (Map.upd m i (Map.sel m i))]
-  = ()
-
-let check_bitmap_for_epoch (#bm:erased _)
-                           (tid_bitmaps: epoch_tid_bitmaps)
-                           (e:M.epoch_id)
-  : ST bool
-    (EpochMap.full_perm tid_bitmaps all_zeroes bm)
-    (fun b -> EpochMap.full_perm tid_bitmaps all_zeroes bm)
-    (requires True)
-    (ensures fun b -> b ==> Map.sel bm e == all_ones)
-  = let res = EpochMap.get tid_bitmaps e in
-    match res with
-    | EpochMap.Found a ->
-      rewrite (EpochMap.get_post all_zeroes bm EpochMap.empty_borrows tid_bitmaps e res)
-              (EpochMap.perm tid_bitmaps all_zeroes bm (PartialMap.upd EpochMap.empty_borrows e a) `star`
-               array_pts_to a (Map.sel bm e));
-      let b = check_all_ones a in
-      EpochMap.ghost_put tid_bitmaps e a _;
-      return b
-
-    | _ ->
-      rewrite (EpochMap.get_post all_zeroes bm EpochMap.empty_borrows tid_bitmaps e res)
-              (EpochMap.full_perm tid_bitmaps all_zeroes bm);
-      return false
-
-
-let check_hash_equality_for_epoch (#hashes_v:erased epoch_hashes_repr)
-                                  (hashes:all_epoch_hashes)
-                                  (e:M.epoch_id)
-  : ST bool
-    (EpochMap.full_perm hashes M.init_epoch_hash hashes_v)
-    (fun _ -> EpochMap.full_perm hashes M.init_epoch_hash hashes_v)
-    (requires True)
-    (ensures fun b ->
-      let ha = Map.sel hashes_v e in
-      b ==> ha.hadd == ha.hevict)
-  = let res = EpochMap.get hashes e in
-    match res with
-    | EpochMap.Found ehs ->
-      rewrite (EpochMap.get_post M.init_epoch_hash hashes_v EpochMap.empty_borrows hashes e res)
-              (EpochMap.perm hashes M.init_epoch_hash hashes_v (PartialMap.upd EpochMap.empty_borrows e ehs) `star`
-               epoch_hash_perm e ehs (Map.sel hashes_v e));
-      rewrite (epoch_hash_perm e ehs (Map.sel hashes_v e)) //TODO: mark epoch_hash_perm reduce
-              (HA.ha_val ehs.hadd (Map.sel hashes_v e).hadd `star`
-               HA.ha_val ehs.hevict (Map.sel hashes_v e).hevict);
-      let b = HA.compare ehs.hadd ehs.hevict in
-      rewrite (HA.ha_val ehs.hadd (Map.sel hashes_v e).hadd `star`
-               HA.ha_val ehs.hevict (Map.sel hashes_v e).hevict)
-              (epoch_hash_perm e ehs (Map.sel hashes_v e));
-      EpochMap.ghost_put hashes e ehs _;
-      return  b
-
-    | _ ->
-      rewrite (EpochMap.get_post M.init_epoch_hash hashes_v EpochMap.empty_borrows hashes e res)
-              (EpochMap.full_perm hashes M.init_epoch_hash hashes_v);
-      return false
-
-let epoch_ready_if_bitmap_set (hashes:epoch_hashes_repr)
-                              (bitmaps:epoch_bitmaps_repr)
-                              (max:_)
-                              (mlogs_v:_)
-                              (e:M.epoch_id)
-  : Lemma
-    (requires
-      hashes_bitmaps_max_ok hashes bitmaps max mlogs_v /\
-      Map.sel bitmaps e == all_ones)
-    (ensures
-      epoch_is_complete mlogs_v e /\
-      Map.sel hashes e == aggregate_all_threads_epoch_hashes e mlogs_v)
-  = ()
 
 let epoch_is_certified (mlogs_v:all_processed_entries)
                        (e:M.epoch_id)
@@ -267,139 +179,7 @@ let max_is_correct (mlogs_v:_) (max:_)
           U32.v e <= U32.v max ==>
           epoch_is_certified mlogs_v e
 
-let _max_is_correct (hashes:_)
-                    (bitmaps:_)
-                    (max:_)
-                    (mlogs_v:_)
-  : Lemma
-    (requires hashes_bitmaps_max_ok hashes bitmaps max mlogs_v)
-    (ensures  max_is_correct mlogs_v max)
-  = ()
-
-
-let try_increment_max (#hashes_v:erased _)
-                      (#bitmaps_v:erased _)
-                      (#mlogs_v:erased _)
-                      (hashes: all_epoch_hashes)
-                      (bitmaps: epoch_tid_bitmaps)
-                      (max:R.ref M.epoch_id)
-  : STT bool
-    (EpochMap.full_perm hashes M.init_epoch_hash hashes_v `star`
-     EpochMap.full_perm bitmaps all_zeroes bitmaps_v `star`
-     exists_ (fun max_v ->
-       R.pts_to max full max_v `star`
-       pure (hashes_bitmaps_max_ok hashes_v bitmaps_v max_v mlogs_v)))
-    (fun b ->
-      EpochMap.full_perm hashes M.init_epoch_hash hashes_v `star`
-      EpochMap.full_perm bitmaps all_zeroes bitmaps_v `star`
-      exists_ (fun (max_v':M.epoch_id) ->
-        R.pts_to max full max_v' `star`
-        pure (hashes_bitmaps_max_ok hashes_v bitmaps_v max_v' mlogs_v)))
-  = let max_v = elim_exists () in
-    let e = R.read max in
-    let v = check_overflow_add32 e 1ul in
-    match v with
-    | None ->
-      intro_exists_erased max_v (fun max_v' ->
-        R.pts_to max full max_v' `star`
-        pure (hashes_bitmaps_max_ok hashes_v bitmaps_v max_v' mlogs_v));
-      return false
-
-    | Some e' ->
-      let ready = check_bitmap_for_epoch bitmaps e' in
-      if not ready
-      then (
-        intro_exists_erased max_v (fun max_v' ->
-          R.pts_to max full max_v' `star`
-          pure (hashes_bitmaps_max_ok hashes_v bitmaps_v max_v' mlogs_v));
-        return false
-      )
-      else (
-        let b = check_hash_equality_for_epoch hashes e' in
-        if not b
-        then (
-          intro_exists_erased max_v (fun max_v' ->
-            R.pts_to max full max_v' `star`
-            pure (hashes_bitmaps_max_ok hashes_v bitmaps_v max_v' mlogs_v));
-          return false
-        )
-        else (
-          R.write max e';
-          elim_pure _;
-          intro_pure (hashes_bitmaps_max_ok hashes_v bitmaps_v e' mlogs_v);
-          intro_exists e' (fun max_v' ->
-            R.pts_to max full max_v' `star`
-            pure (hashes_bitmaps_max_ok hashes_v bitmaps_v max_v' mlogs_v));
-           return true
-        )
-      )
-
-let try_advance_max (#hashes_v:erased epoch_hashes_repr)
-                    (#bitmaps_v:erased epoch_bitmaps_repr)
-                    (#max_v:erased _)
-                    (#mlogs_v:erased _)
-                    (hashes: all_epoch_hashes)
-                    (bitmaps: epoch_tid_bitmaps)
-                    (max:R.ref M.epoch_id)
-  : STT M.epoch_id
-    (EpochMap.full_perm hashes M.init_epoch_hash hashes_v `star`
-     EpochMap.full_perm bitmaps all_zeroes bitmaps_v `star`
-     R.pts_to max full max_v `star`
-     pure (hashes_bitmaps_max_ok hashes_v bitmaps_v max_v mlogs_v))
-    (fun max_v' ->
-      EpochMap.full_perm hashes M.init_epoch_hash hashes_v `star`
-      EpochMap.full_perm bitmaps all_zeroes bitmaps_v `star`
-      R.pts_to max full max_v' `star`
-      pure (hashes_bitmaps_max_ok hashes_v bitmaps_v max_v' mlogs_v))
-  = intro_exists_erased max_v (fun max_v ->
-       R.pts_to max full max_v `star`
-       pure (hashes_bitmaps_max_ok hashes_v bitmaps_v max_v mlogs_v));
-    repeat_until _ (fun _ -> try_increment_max #hashes_v #bitmaps_v #mlogs_v hashes bitmaps max);
-    let _ = elim_exists _ in
-    let max = R.read max in
-    elim_pure _;
-    intro_pure _;
-    return max
-
-let release_lock (#hv:erased epoch_hashes_repr)
-                 (#bitmaps:erased epoch_bitmaps_repr)
-                 (#max:erased _)
-                 (#mlogs_v:erased _)
-                 (#hashes : all_epoch_hashes)
-                 (#tid_bitmaps : epoch_tid_bitmaps)
-                 (#max_certified_epoch : R.ref M.epoch_id)
-                 (#mlogs: TLM.t)
-                 (lock: cancellable_lock
-                        (lock_inv hashes tid_bitmaps max_certified_epoch mlogs))
-  : STT unit
-    (lock_inv_body hashes tid_bitmaps max_certified_epoch mlogs
-                       hv bitmaps max mlogs_v `star`
-     can_release lock)
-    (fun _ -> emp)
-  = intro_exists_erased mlogs_v
-      (fun mlogs_v ->  lock_inv_body hashes tid_bitmaps max_certified_epoch mlogs
-                                      hv bitmaps max mlogs_v);
-    intro_exists_erased max
-      (fun max ->
-        exists_ (fun mlogs_v ->
-                    lock_inv_body hashes tid_bitmaps max_certified_epoch mlogs
-                                      hv bitmaps max mlogs_v));
-    intro_exists_erased bitmaps
-      (fun bitmaps ->
-        exists_ (fun max ->
-        exists_ (fun mlogs_v ->
-                    lock_inv_body hashes tid_bitmaps max_certified_epoch mlogs
-                                      hv bitmaps max mlogs_v)));
-    intro_exists_erased hv
-      (fun hv ->
-        exists_ (fun bitmaps ->
-        exists_ (fun max ->
-        exists_ (fun mlogs_v ->
-                    lock_inv_body hashes tid_bitmaps max_certified_epoch mlogs
-                                      hv bitmaps max mlogs_v))));
-    release lock
-
-let advance_and_read_max_certified_epoch (aeh:aggregate_epoch_hashes)
+val advance_and_read_max_certified_epoch (aeh:aggregate_epoch_hashes)
   : STT (option M.epoch_id)
       emp
       (fun max_opt ->
@@ -409,45 +189,3 @@ let advance_and_read_max_certified_epoch (aeh:aggregate_epoch_hashes)
           exists_ (fun logs ->
            TLM.global_snapshot aeh.mlogs (map_of_seq logs) `star`
            pure (max_is_correct logs max)))
-  = let b = acquire aeh.lock in
-    if not b
-    then (
-      rewrite (maybe_acquired _ _)
-              emp;
-      return None
-    )
-    else (
-      rewrite (maybe_acquired _ _)
-              (lock_inv aeh.hashes
-                        aeh.tid_bitmaps
-                        aeh.max_certified_epoch
-                        aeh.mlogs `star`
-              can_release aeh.lock);
-      let _hv = elim_exists () in
-      let _bitmaps = elim_exists () in
-      let _max = elim_exists () in
-      let _mlogs_v : erased all_processed_entries =
-          elim_exists #_ #_
-            #(lock_inv_body
-                 aeh.hashes
-                 aeh.tid_bitmaps
-                 aeh.max_certified_epoch
-                 aeh.mlogs
-                 _hv
-                 _bitmaps
-                 _max)
-            ()
-      in
-
-      let max = try_advance_max aeh.hashes aeh.tid_bitmaps aeh.max_certified_epoch in
-      extract_pure _;
-
-      intro_pure (max_is_correct _mlogs_v max);
-      TLM.take_snapshot aeh.mlogs (map_of_seq _mlogs_v);
-      intro_exists_erased _mlogs_v
-        (fun logs ->
-           TLM.global_snapshot aeh.mlogs (map_of_seq logs) `star`
-           pure (max_is_correct logs max));
-      release_lock #_ #_ #(hide max) aeh.lock;
-      return (Some max)
-    )
